% Created using perl make-latex.pl "x*dy"

\documentclass{amsart}

\begin{document}

\allowdisplaybreaks[4]

Output of {\tt expand-method.pl} applied to {\tt x*dy}.

\begin{align*}
c_{l,l-2}^{m,m-2} &= -\frac{i(l+1)\sqrt{l+m-3}\sqrt{l+m-2}\sqrt{l+m-1}\sqrt{l+m}}{4\sqrt{2l-3}(2l-1)\sqrt{2l+1}} \\
c_{l,l-2}^{m,m+2} &= \frac{i(l+1)\sqrt{l-m-3}\sqrt{l-m-2}\sqrt{l-m-1}\sqrt{l-m}}{4\sqrt{2l-3}(2l-1)\sqrt{2l+1}} \\
c_{l,l}^{m,m-2} &= \frac{3i\sqrt{l-m+1}\sqrt{l-m+2}\sqrt{l+m-1}\sqrt{l+m}}{4\left(4l^2+4l-3\right)} \\
c_{l,l}^{m,m} &= -\frac{im}{2} \\
c_{l,l}^{m,m+2} &= -\frac{3i\sqrt{l-m-1}\sqrt{l-m}\sqrt{l+m+1}\sqrt{l+m+2}}{4\left(4l^2+4l-3\right)} \\
c_{l,l+2}^{m,m-2} &= \frac{il\sqrt{l-m+1}\sqrt{l-m+2}\sqrt{l-m+3}\sqrt{l-m+4}}{\sqrt{2l+1}\sqrt{2l+5}(8l+12)} \\
c_{l,l+2}^{m,m+2} &= -\frac{il\sqrt{l+m+1}\sqrt{l+m+2}\sqrt{l+m+3}\sqrt{l+m+4}}{\sqrt{2l+1}\sqrt{2l+5}(8l+12)}
\end{align*}

\end{document}
