\documentclass{amsart}

\usepackage{amssymb,amsmath}

\begin{document}

\noindent
``op'' denotes any of $z$, $iL_z$, $L_+$, or $L_-$, and $\mathcal Y$ denotes any linear combination of the $\bar Y_l^m$'s.
\begin{align*}
\text{op}(\mathcal Y \pm c \bar Y_l^m) &\to \text{op}(\mathcal Y) \pm c \, \text{op}(\bar Y_l^m) \\
x \mathcal Y &\to  z iL_y(\mathcal Y) - i L_y(z\mathcal Y) \\
y \mathcal Y &\to  i L_x(z\mathcal Y) - z iL_x(\mathcal Y) \\
z\bar Y_l^m &\to \sqrt{\frac{(l+m)(l-m)}{(2l-1)(2l+1)}} \bar Y_{l-1}^m + \sqrt{\frac{(l+m+1)(l-m+1)}{(2l+1)(2l+3)}} \bar Y_{l+1}^m \\
\nabla_x \mathcal Y &\to z i L_y(\mathcal Y) - y i L_z(\mathcal Y)  \\
\nabla_y \mathcal Y &\to x i L_z(\mathcal Y) - z i L_x(\mathcal Y)  \\
\nabla_z \mathcal Y &\to y i L_x(\mathcal Y) - x i L_y(\mathcal Y)  \\
iL_x (\mathcal Y) &\to \tfrac i2 \left(L_+ (\mathcal Y) + L_- (\mathcal Y)\right) \\
iL_y (\mathcal Y) &\to \tfrac 12 \left(L_+ (\mathcal Y) - L_- (\mathcal Y)\right) \\
i L_z \bar Y_l^m &\to -im\bar Y_l^m \\
L_+ \bar Y_l^m &\to - \sqrt{(l+m)(l-m+1)}\bar Y_l^{m-1} \\
L_- \bar Y_l^m &\to - \sqrt{(l-m)(l+m+1)}\bar Y_l^{m+1}
\end{align*}

\end{document}
